<?xml version="1.0"?>
<rdf:RDF xmlns="http://www.w3.org/2002/07/owl#"
     xml:base="http://www.w3.org/2002/07/owl"
     xmlns:owl="http://www.w3.org/2002/07/owl#"
     xmlns:rdf="http://www.w3.org/1999/02/22-rdf-syntax-ns#"
     xmlns:xml="http://www.w3.org/XML/1998/namespace"
     xmlns:xsd="http://www.w3.org/2001/XMLSchema#"
     xmlns:hdf5="http://purl.allotrope.org/ontologies/hdf5/1.8#"
     xmlns:owl1="https://www.w3.org/2002/07/owl#"
     xmlns:rdfs="http://www.w3.org/2000/01/rdf-schema#"
     xmlns:skos="http://www.w3.org/2004/02/skos/core#"
     xmlns:ssno="https://matthiasprobst.github.io/ssno#"
     xmlns:vann="http://purl.org/vocab/vann/"
     xmlns:terms="http://purl.org/dc/terms/"
     xmlns:rdf-syntax-ns="https://www.w3.org/1999/02/22-rdf-syntax-ns#">
    <Ontology/>
    


    <!-- 
    ///////////////////////////////////////////////////////////////////////////////////////
    //
    // Annotation properties
    //
    ///////////////////////////////////////////////////////////////////////////////////////
     -->


    


    <!-- http://purl.allotrope.org/ontologies/hdf5/1.8#rootGroup -->


    <AnnotationProperty rdf:about="http://purl.allotrope.org/ontologies/hdf5/1.8#rootGroup">
        <rdfs:isDefinedBy rdf:resource="http://purl.allotrope.org/ontologies/hdf5/1.8#"/>
        <skos:definition xml:lang="en">Relation between the HDF file and its root group</skos:definition>
        <skos:prefLabel xml:lang="en">has root group</skos:prefLabel>
        <rdf-syntax-ns:type rdf:resource="https://www.w3.org/2002/07/owl#ObjectProperty"/>
        <rdfs:domain rdf:resource="http://purl.allotrope.org/ontologies/hdf5/1.8#File"/>
    </AnnotationProperty>
    


    <!-- http://purl.org/dc/terms/abstract -->


    <AnnotationProperty rdf:about="http://purl.org/dc/terms/abstract">
        <rdf-syntax-ns:type rdf:resource="https://www.w3.org/2002/07/owl#AnnotationProperty"/>
    </AnnotationProperty>
    


    <!-- http://purl.org/dc/terms/created -->


    <AnnotationProperty rdf:about="http://purl.org/dc/terms/created">
        <rdf-syntax-ns:type rdf:resource="https://www.w3.org/2002/07/owl#AnnotationProperty"/>
    </AnnotationProperty>
    


    <!-- http://purl.org/dc/terms/creator -->


    <AnnotationProperty rdf:about="http://purl.org/dc/terms/creator">
        <rdf-syntax-ns:type rdf:resource="https://www.w3.org/2002/07/owl#AnnotationProperty"/>
    </AnnotationProperty>
    


    <!-- http://purl.org/dc/terms/license -->


    <AnnotationProperty rdf:about="http://purl.org/dc/terms/license">
        <rdf-syntax-ns:type rdf:resource="https://www.w3.org/2002/07/owl#AnnotationProperty"/>
    </AnnotationProperty>
    


    <!-- http://purl.org/dc/terms/rights -->


    <AnnotationProperty rdf:about="http://purl.org/dc/terms/rights">
        <rdf-syntax-ns:type rdf:resource="https://www.w3.org/2002/07/owl#AnnotationProperty"/>
    </AnnotationProperty>
    


    <!-- http://purl.org/vocab/vann/preferredNamespacePrefix -->


    <AnnotationProperty rdf:about="http://purl.org/vocab/vann/preferredNamespacePrefix">
        <rdf-syntax-ns:type rdf:resource="https://www.w3.org/2002/07/owl#AnnotationProperty"/>
    </AnnotationProperty>
    


    <!-- http://purl.org/vocab/vann/preferredNamespaceUri -->


    <AnnotationProperty rdf:about="http://purl.org/vocab/vann/preferredNamespaceUri">
        <rdf-syntax-ns:type rdf:resource="https://www.w3.org/2002/07/owl#AnnotationProperty"/>
    </AnnotationProperty>
    


    <!-- http://www.w3.org/2001/XMLSchema#pattern -->


    <AnnotationProperty rdf:about="http://www.w3.org/2001/XMLSchema#pattern"/>
    


    <!-- http://www.w3.org/2004/02/skos/core#closeMatch -->


    <AnnotationProperty rdf:about="http://www.w3.org/2004/02/skos/core#closeMatch">
        <rdf-syntax-ns:type rdf:resource="https://www.w3.org/2002/07/owl#AnnotationProperty"/>
    </AnnotationProperty>
    


    <!-- http://www.w3.org/2004/02/skos/core#definition -->


    <AnnotationProperty rdf:about="http://www.w3.org/2004/02/skos/core#definition">
        <rdf-syntax-ns:type rdf:resource="https://www.w3.org/2002/07/owl#AnnotationProperty"/>
    </AnnotationProperty>
    


    <!-- http://www.w3.org/2004/02/skos/core#example -->


    <AnnotationProperty rdf:about="http://www.w3.org/2004/02/skos/core#example">
        <rdf-syntax-ns:type rdf:resource="https://www.w3.org/2002/07/owl#AnnotationProperty"/>
    </AnnotationProperty>
    


    <!-- http://www.w3.org/2004/02/skos/core#prefLabel -->


    <AnnotationProperty rdf:about="http://www.w3.org/2004/02/skos/core#prefLabel">
        <rdf-syntax-ns:type rdf:resource="https://www.w3.org/2002/07/owl#AnnotationProperty"/>
    </AnnotationProperty>
    


    <!-- https://matthiasprobst.github.io/ssno#after -->


    <AnnotationProperty rdf:about="https://matthiasprobst.github.io/ssno#after">
        <rdfs:subPropertyOf rdf:resource="https://matthiasprobst.github.io/ssno#positioned"/>
    </AnnotationProperty>
    


    <!-- https://matthiasprobst.github.io/ssno#before -->


    <AnnotationProperty rdf:about="https://matthiasprobst.github.io/ssno#before">
        <rdfs:subPropertyOf rdf:resource="https://matthiasprobst.github.io/ssno#positioned"/>
    </AnnotationProperty>
    


    <!-- https://matthiasprobst.github.io/ssno#positioned -->


    <AnnotationProperty rdf:about="https://matthiasprobst.github.io/ssno#positioned">
        <skos:definition xml:lang="en">Relates two qualifications or one qualification and a standard name to each other.</skos:definition>
        <skos:prefLabel xml:lang="en">positioned</skos:prefLabel>
        <rdf-syntax-ns:type rdf:resource="https://www.w3.org/2002/07/owl#ObjectProperty"/>
        <rdf-syntax-ns:type rdf:resource="https://www.w3.org/2002/07/owl#TransitiveProperty"/>
    </AnnotationProperty>
    


    <!-- https://www.w3.org/1999/02/22-rdf-syntax-ns#type -->


    <AnnotationProperty rdf:about="https://www.w3.org/1999/02/22-rdf-syntax-ns#type"/>
    


    <!-- https://www.w3.org/2002/07/owl#cardinality -->


    <AnnotationProperty rdf:about="https://www.w3.org/2002/07/owl#cardinality"/>
    


    <!-- https://www.w3.org/2002/07/owl#disjointWith -->


    <AnnotationProperty rdf:about="https://www.w3.org/2002/07/owl#disjointWith"/>
    


    <!-- https://www.w3.org/2002/07/owl#equivalentClass -->


    <AnnotationProperty rdf:about="https://www.w3.org/2002/07/owl#equivalentClass"/>
    


    <!-- https://www.w3.org/2002/07/owl#inverseOf -->


    <AnnotationProperty rdf:about="https://www.w3.org/2002/07/owl#inverseOf"/>
    


    <!-- https://www.w3.org/2002/07/owl#maxQualifiedCardinality -->


    <AnnotationProperty rdf:about="https://www.w3.org/2002/07/owl#maxQualifiedCardinality"/>
    


    <!-- https://www.w3.org/2002/07/owl#minQualifiedCardinality -->


    <AnnotationProperty rdf:about="https://www.w3.org/2002/07/owl#minQualifiedCardinality"/>
    


    <!-- https://www.w3.org/2002/07/owl#onClass -->


    <AnnotationProperty rdf:about="https://www.w3.org/2002/07/owl#onClass"/>
    


    <!-- https://www.w3.org/2002/07/owl#onDataRange -->


    <AnnotationProperty rdf:about="https://www.w3.org/2002/07/owl#onDataRange"/>
    


    <!-- https://www.w3.org/2002/07/owl#onDatatype -->


    <AnnotationProperty rdf:about="https://www.w3.org/2002/07/owl#onDatatype"/>
    


    <!-- https://www.w3.org/2002/07/owl#onProperty -->


    <AnnotationProperty rdf:about="https://www.w3.org/2002/07/owl#onProperty"/>
    


    <!-- https://www.w3.org/2002/07/owl#qualifiedCardinality -->


    <AnnotationProperty rdf:about="https://www.w3.org/2002/07/owl#qualifiedCardinality"/>
    


    <!-- https://www.w3.org/2002/07/owl#someValuesFrom -->


    <AnnotationProperty rdf:about="https://www.w3.org/2002/07/owl#someValuesFrom"/>
    


    <!-- https://www.w3.org/2002/07/owl#unionOf -->


    <AnnotationProperty rdf:about="https://www.w3.org/2002/07/owl#unionOf"/>
    


    <!-- https://www.w3.org/2002/07/owl#versionIRI -->


    <AnnotationProperty rdf:about="https://www.w3.org/2002/07/owl#versionIRI"/>
    


    <!-- https://www.w3.org/2002/07/owl#versionInfo -->


    <AnnotationProperty rdf:about="https://www.w3.org/2002/07/owl#versionInfo"/>
    


    <!-- https://www.w3.org/2002/07/owl#withRestrictions -->


    <AnnotationProperty rdf:about="https://www.w3.org/2002/07/owl#withRestrictions"/>
    


    <!-- 
    ///////////////////////////////////////////////////////////////////////////////////////
    //
    // Datatypes
    //
    ///////////////////////////////////////////////////////////////////////////////////////
     -->


    


    <!-- http://org.semanticweb.owlapi/error#Error7 -->


    <rdfs:Datatype rdf:about="http://org.semanticweb.owlapi/error#Error7"/>
    


    <!-- 
    ///////////////////////////////////////////////////////////////////////////////////////
    //
    // Object Properties
    //
    ///////////////////////////////////////////////////////////////////////////////////////
     -->


    


    <!-- http://purl.allotrope.org/ontologies/hdf5/1.8#member -->


    <ObjectProperty rdf:about="http://purl.allotrope.org/ontologies/hdf5/1.8#member">
        <rdfs:domain rdf:resource="http://purl.allotrope.org/ontologies/hdf5/1.8#Group"/>
        <rdfs:range rdf:resource="http://org.semanticweb.owlapi/error#Error3"/>
        <skos:definition xml:lang="en">Relation between collection and the members of it.</skos:definition>
        <skos:prefLabel xml:lang="en">member</skos:prefLabel>
        <rdf-syntax-ns:type rdf:resource="https://www.w3.org/2002/07/owl#ObjectProperty"/>
    </ObjectProperty>
    


    <!-- http://www.w3.org/ns/dcat#hadRole -->


    <ObjectProperty rdf:about="http://www.w3.org/ns/dcat#hadRole">
        <rdfs:domain rdf:resource="http://www.w3.org/ns/prov#Attribution"/>
        <rdfs:range rdf:resource="http://www.w3.org/ns/dcat#Role"/>
        <rdfs:comment xml:lang="en">This DCAT property complements prov:hadRole which provides the function of an entity or agent with respect to an activity.</rdfs:comment>
        <skos:definition xml:lang="en">The function of an entity or agent with respect to another entity or resource.</skos:definition>
        <skos:prefLabel xml:lang="en">had role</skos:prefLabel>
        <rdf-syntax-ns:type rdf:resource="https://www.w3.org/2002/07/owl#ObjectProperty"/>
    </ObjectProperty>
    


    <!-- http://www.w3.org/ns/prov#agent -->


    <ObjectProperty rdf:about="http://www.w3.org/ns/prov#agent">
        <rdfs:domain rdf:resource="http://www.w3.org/ns/prov#Attribution"/>
        <rdfs:range rdf:resource="http://www.w3.org/ns/prov#Agent"/>
        <skos:definition xml:lang="en">The prov:agent property references an prov:Agent which influenced a resource. This property applies to an prov:AgentInfluence, which is given by a subproperty of prov:qualifiedInfluence from the influenced prov:Entity, prov:Activity or prov:Agent.</skos:definition>
        <skos:prefLabel xml:lang="en">agent</skos:prefLabel>
        <rdf-syntax-ns:type rdf:resource="https://www.w3.org/2002/07/owl#ObjectProperty"/>
    </ObjectProperty>
    


    <!-- http://www.w3.org/ns/prov#qualifiedAttribution -->


    <ObjectProperty rdf:about="http://www.w3.org/ns/prov#qualifiedAttribution">
        <rdfs:domain rdf:resource="http://www.w3.org/ns/dcat#Dataset"/>
        <rdfs:range rdf:resource="http://www.w3.org/ns/prov#Attribution"/>
        <skos:definition xml:lang="en">Attribution is the ascribing of an entity to an agent. When an entity e is attributed to agent ag, entity e was generated by some unspecified activity that in turn was associated to agent ag. Thus, this relation is useful when the activity is not known, or irrelevant</skos:definition>
        <skos:prefLabel xml:lang="en">qualified attribution</skos:prefLabel>
        <rdf-syntax-ns:type rdf:resource="https://www.w3.org/2002/07/owl#ObjectProperty"/>
    </ObjectProperty>
    


    <!-- https://matthiasprobst.github.io/ssno#after -->


    <ObjectProperty rdf:about="https://matthiasprobst.github.io/ssno#after">
        <rdfs:domain rdf:resource="https://matthiasprobst.github.io/ssno#Qualification"/>
        <rdfs:range rdf:resource="http://org.semanticweb.owlapi/error#Error9"/>
    </ObjectProperty>
    


    <!-- https://matthiasprobst.github.io/ssno#alias -->


    <ObjectProperty rdf:about="https://matthiasprobst.github.io/ssno#alias">
        <rdfs:domain rdf:resource="https://matthiasprobst.github.io/ssno#StandardName"/>
        <rdfs:range rdf:resource="https://matthiasprobst.github.io/ssno#StandardName"/>
        <skos:definition xml:lang="en">Indicates that a standard name individual is an alias of another.</skos:definition>
        <skos:prefLabel xml:lang="en">alias</skos:prefLabel>
        <rdf-syntax-ns:type rdf:resource="https://www.w3.org/2002/07/owl#ObjectProperty"/>
        <rdf-syntax-ns:type rdf:resource="https://www.w3.org/2002/07/owl#TransitiveProperty"/>
    </ObjectProperty>
    


    <!-- https://matthiasprobst.github.io/ssno#associatedWith -->


    <ObjectProperty rdf:about="https://matthiasprobst.github.io/ssno#associatedWith">
        <rdfs:domain rdf:resource="https://matthiasprobst.github.io/ssno#Character"/>
        <rdfs:range rdf:resource="http://org.semanticweb.owlapi/error#Error2"/>
        <skos:definition xml:lang="en">Associates a character to a thing, which is intended to be a AnyStandardName or a Qualification.</skos:definition>
        <skos:prefLabel xml:lang="en">associated with</skos:prefLabel>
        <rdf-syntax-ns:type rdf:resource="https://www.w3.org/2002/07/owl#ObjectProperty"/>
    </ObjectProperty>
    


    <!-- https://matthiasprobst.github.io/ssno#before -->


    <ObjectProperty rdf:about="https://matthiasprobst.github.io/ssno#before">
        <rdfs:domain rdf:resource="https://matthiasprobst.github.io/ssno#Qualification"/>
        <rdfs:range rdf:resource="http://org.semanticweb.owlapi/error#Error6"/>
    </ObjectProperty>
    


    <!-- https://matthiasprobst.github.io/ssno#description -->


    <ObjectProperty rdf:about="https://matthiasprobst.github.io/ssno#description">
        <rdfs:domain rdf:resource="http://org.semanticweb.owlapi/error#Error21"/>
        <rdfs:range rdf:resource="http://org.semanticweb.owlapi/error#Error10"/>
    </ObjectProperty>
    


    <!-- https://matthiasprobst.github.io/ssno#hasCharacter -->


    <ObjectProperty rdf:about="https://matthiasprobst.github.io/ssno#hasCharacter">
        <rdfs:domain rdf:resource="https://matthiasprobst.github.io/ssno#Transformation"/>
        <rdfs:range rdf:resource="https://matthiasprobst.github.io/ssno#Character"/>
        <skos:definition xml:lang="en">Links a transformation to a character used in the transformation string to represent a standard name or qualification</skos:definition>
        <skos:prefLabel xml:lang="en">has character</skos:prefLabel>
        <rdf-syntax-ns:type rdf:resource="https://www.w3.org/2002/07/owl#ObjectProperty"/>
    </ObjectProperty>
    


    <!-- https://matthiasprobst.github.io/ssno#hasModifier -->


    <ObjectProperty rdf:about="https://matthiasprobst.github.io/ssno#hasModifier">
        <rdfs:domain rdf:resource="https://matthiasprobst.github.io/ssno#StandardNameTable"/>
        <rdfs:range rdf:resource="http://org.semanticweb.owlapi/error#Error4"/>
        <skos:definition xml:lang="en">Points to a Qualification or Transformation defined by a Standard Name Table</skos:definition>
        <skos:prefLabel xml:lang="en">has modifier</skos:prefLabel>
        <rdf-syntax-ns:type rdf:resource="https://www.w3.org/2002/07/owl#ObjectProperty"/>
    </ObjectProperty>
    


    <!-- https://matthiasprobst.github.io/ssno#hasStandardName -->


    <ObjectProperty rdf:about="https://matthiasprobst.github.io/ssno#hasStandardName">
        <rdfs:domain rdf:resource="http://org.semanticweb.owlapi/error#Error18"/>
        <rdfs:range rdf:resource="https://matthiasprobst.github.io/ssno#StandardName"/>
        <skos:definition xml:lang="en">Points to a ssno:StandardName associated with the Concept. The Concept should is expected to be describing a numerical quantity because a ssno:StandardName defines and describe a numerical quantity by providing a description and expected canonical unit.</skos:definition>
        <skos:prefLabel xml:lang="en">has standard name</skos:prefLabel>
        <rdf-syntax-ns:type rdf:resource="https://www.w3.org/2002/07/owl#ObjectProperty"/>
        <owl1:inverseOf rdf:resource="https://matthiasprobst.github.io/ssno#isStandardNameOf"/>
    </ObjectProperty>
    


    <!-- https://matthiasprobst.github.io/ssno#hasValidValues -->


    <ObjectProperty rdf:about="https://matthiasprobst.github.io/ssno#hasValidValues">
        <rdfs:domain rdf:resource="https://matthiasprobst.github.io/ssno#Qualification"/>
        <rdfs:range rdf:resource="http://w3id.org/nfdi4ing/metadata4ing#TextVariable"/>
        <skos:definition xml:lang="en">A relationship defining a set of values used by the qualification.</skos:definition>
        <skos:prefLabel xml:lang="en">has valid values</skos:prefLabel>
        <rdf-syntax-ns:type rdf:resource="https://www.w3.org/2002/07/owl#ObjectProperty"/>
    </ObjectProperty>
    


    <!-- https://matthiasprobst.github.io/ssno#isStandardNameOf -->


    <ObjectProperty rdf:about="https://matthiasprobst.github.io/ssno#isStandardNameOf">
        <rdfs:domain rdf:resource="https://matthiasprobst.github.io/ssno#StandardName"/>
        <rdfs:range rdf:resource="http://org.semanticweb.owlapi/error#Error1"/>
        <skos:definition xml:lang="en">Points to a Concept, that describes a numerical variable, which uses the standard name.</skos:definition>
        <skos:prefLabel xml:lang="en">is standard name of</skos:prefLabel>
        <rdf-syntax-ns:type rdf:resource="https://www.w3.org/2002/07/owl#ObjectProperty"/>
    </ObjectProperty>
    


    <!-- https://matthiasprobst.github.io/ssno#standardNameTable -->


    <ObjectProperty rdf:about="https://matthiasprobst.github.io/ssno#standardNameTable">
        <rdfs:domain rdf:resource="https://matthiasprobst.github.io/ssno#StandardName"/>
        <rdfs:range rdf:resource="http://org.semanticweb.owlapi/error#Error11"/>
        <skos:definition xml:lang="en">Points to the ssno:StandardNameTable defining the ssno:StandardName.</skos:definition>
        <skos:prefLabel xml:lang="en">standard name table</skos:prefLabel>
        <rdf-syntax-ns:type rdf:resource="https://www.w3.org/2002/07/owl#ObjectProperty"/>
        <owl1:inverseOf rdf:resource="https://matthiasprobst.github.io/ssno#standardNames"/>
    </ObjectProperty>
    


    <!-- https://matthiasprobst.github.io/ssno#standardNameTableUsedBy -->


    <ObjectProperty rdf:about="https://matthiasprobst.github.io/ssno#standardNameTableUsedBy">
        <rdfs:domain rdf:resource="https://matthiasprobst.github.io/ssno#StandardNameTable"/>
        <rdfs:range rdf:resource="http://org.semanticweb.owlapi/error#Error8"/>
        <skos:definition xml:lang="en">Points to a concept, which uses a standard name table.</skos:definition>
        <skos:prefLabel xml:lang="en">standard name table used by</skos:prefLabel>
        <rdf-syntax-ns:type rdf:resource="https://www.w3.org/2002/07/owl#ObjectProperty"/>
        <owl1:inverseOf rdf:resource="https://matthiasprobst.github.io/ssno#usesStandardNameTable"/>
    </ObjectProperty>
    


    <!-- https://matthiasprobst.github.io/ssno#standardNames -->


    <ObjectProperty rdf:about="https://matthiasprobst.github.io/ssno#standardNames">
        <rdfs:domain rdf:resource="https://matthiasprobst.github.io/ssno#StandardNameTable"/>
        <rdfs:range rdf:resource="https://matthiasprobst.github.io/ssno#StandardName"/>
        <skos:definition xml:lang="en">Points to one or more scalar or vector standard names defined in a standard name table.</skos:definition>
        <skos:prefLabel xml:lang="en">standard names</skos:prefLabel>
        <rdf-syntax-ns:type rdf:resource="https://www.w3.org/2002/07/owl#ObjectProperty"/>
    </ObjectProperty>
    


    <!-- https://matthiasprobst.github.io/ssno#unit -->


    <ObjectProperty rdf:about="https://matthiasprobst.github.io/ssno#unit">
        <rdfs:domain rdf:resource="https://matthiasprobst.github.io/ssno#StandardName"/>
        <rdfs:range rdf:resource="http://qudt.org/schema/qudt/Unit"/>
        <skos:closeMatch rdf:resource="http://qudt.org/schema/qudt/unit"/>
        <skos:closeMatch rdf:resource="http://w3id.org/nfdi4ing/metadata4ing#hasUnit"/>
        <skos:closeMatch rdf:resource="https://ptb.de/si/hasUnit"/>
        <skos:definition xml:lang="en">The unit of the standard name. The unit of an individual standard name must be convertable to this unit.</skos:definition>
        <skos:prefLabel xml:lang="en">unit</skos:prefLabel>
        <rdf-syntax-ns:type rdf:resource="https://www.w3.org/2002/07/owl#FunctionalProperty"/>
        <rdf-syntax-ns:type rdf:resource="https://www.w3.org/2002/07/owl#ObjectProperty"/>
    </ObjectProperty>
    


    <!-- https://matthiasprobst.github.io/ssno#usesStandardNameTable -->


    <ObjectProperty rdf:about="https://matthiasprobst.github.io/ssno#usesStandardNameTable">
        <rdfs:domain rdf:resource="http://org.semanticweb.owlapi/error#Error13"/>
        <rdfs:range rdf:resource="http://org.semanticweb.owlapi/error#Error5"/>
        <skos:definition xml:lang="en">Relates a thing, e.g. a netCDF4 file, an HDF5 file or another resource to a standard name table which is associated to the standard names used in the file.</skos:definition>
        <skos:prefLabel xml:lang="en">uses standard name table</skos:prefLabel>
        <rdf-syntax-ns:type rdf:resource="https://www.w3.org/2002/07/owl#ObjectProperty"/>
    </ObjectProperty>
    


    <!-- 
    ///////////////////////////////////////////////////////////////////////////////////////
    //
    // Data properties
    //
    ///////////////////////////////////////////////////////////////////////////////////////
     -->


    


    <!-- http://purl.org/dc/terms/description -->


    <DatatypeProperty rdf:about="http://purl.org/dc/terms/description">
        <rdfs:domain rdf:resource="https://matthiasprobst.github.io/ssno#StandardNameTable"/>
        <rdfs:range rdf:resource="http://www.w3.org/2000/01/rdf-schema#Literal"/>
        <rdf-syntax-ns:type rdf:resource="https://www.w3.org/2002/07/owl#AnnotationProperty"/>
    </DatatypeProperty>
    


    <!-- http://purl.org/dc/terms/hasVersion -->


    <DatatypeProperty rdf:about="http://purl.org/dc/terms/hasVersion">
        <rdfs:domain rdf:resource="https://matthiasprobst.github.io/ssno#StandardNameTable"/>
        <rdfs:range rdf:resource="http://www.w3.org/2000/01/rdf-schema#Literal"/>
        <skos:definition xml:lang="en">A related resource that is a version, edition, or adaptation of the described resource.</skos:definition>
        <skos:prefLabel xml:lang="en">has version</skos:prefLabel>
        <rdf-syntax-ns:type rdf:resource="https://www.w3.org/2002/07/owl#DatatypeProperty"/>
    </DatatypeProperty>
    


    <!-- http://purl.org/dc/terms/identifier -->


    <DatatypeProperty rdf:about="http://purl.org/dc/terms/identifier">
        <rdfs:domain rdf:resource="https://matthiasprobst.github.io/ssno#StandardNameTable"/>
        <rdfs:range rdf:resource="http://www.w3.org/2001/XMLSchema#string"/>
        <rdfs:comment>Recommended practice is to identify the resource by means of a string conforming to an identification system. Examples include International Standard Book Number (ISBN), Digital Object Identifier (DOI), and Uniform Resource Name (URN). Persistent identifiers should be provided as HTTP URIs.</rdfs:comment>
        <rdfs:isDefinedBy rdf:resource="http://purl.org/dc/terms/"/>
        <skos:prefLabel xml:lang="en">identifier</skos:prefLabel>
        <rdf-syntax-ns:type rdf:resource="https://www.w3.org/2002/07/owl#DatatypeProperty"/>
    </DatatypeProperty>
    


    <!-- http://purl.org/dc/terms/subject -->


    <DatatypeProperty rdf:about="http://purl.org/dc/terms/subject">
        <rdfs:domain rdf:resource="https://matthiasprobst.github.io/ssno#StandardNameTable"/>
        <rdfs:range rdf:resource="http://www.w3.org/2001/XMLSchema#string"/>
        <rdfs:comment xml:lang="en">Recommended practice is to refer to the subject with a URI. If this is not possible or feasible, a literal value that identifies the subject may be provided. Both should preferably refer to a subject in a controlled vocabulary.</rdfs:comment>
        <skos:definition xml:lang="en">A topic of the resource.</skos:definition>
        <skos:prefLabel xml:lang="en">subject</skos:prefLabel>
        <rdf-syntax-ns:type rdf:resource="https://www.w3.org/2002/07/owl#AnnotationProperty"/>
    </DatatypeProperty>
    


    <!-- http://purl.org/dc/terms/title -->


    <DatatypeProperty rdf:about="http://purl.org/dc/terms/title">
        <rdfs:domain rdf:resource="https://matthiasprobst.github.io/ssno#StandardNameTable"/>
        <rdfs:range rdf:resource="http://www.w3.org/2001/XMLSchema#anyURI"/>
        <rdf-syntax-ns:type rdf:resource="https://www.w3.org/2002/07/owl#AnnotationProperty"/>
    </DatatypeProperty>
    


    <!-- http://w3id.org/nfdi4ing/metadata4ing#hasRorId -->


    <DatatypeProperty rdf:about="http://w3id.org/nfdi4ing/metadata4ing#hasRorId">
        <rdfs:subPropertyOf rdf:resource="http://w3id.org/nfdi4ing/metadata4ing#identifier"/>
        <rdfs:domain rdf:resource="http://www.w3.org/ns/prov#Organization"/>
        <rdfs:range rdf:resource="http://org.semanticweb.owlapi/error#Error7"/>
        <skos:definition xml:lang="en">A Research Organization Registry identifier, that points to a research organization</skos:definition>
        <skos:prefLabel xml:lang="en">has ROR ID</skos:prefLabel>
        <rdf-syntax-ns:type rdf:resource="https://www.w3.org/2002/07/owl#DatatypeProperty"/>
    </DatatypeProperty>
    


    <!-- http://w3id.org/nfdi4ing/metadata4ing#hasStringValue -->


    <DatatypeProperty rdf:about="http://w3id.org/nfdi4ing/metadata4ing#hasStringValue">
        <rdfs:domain rdf:resource="http://w3id.org/nfdi4ing/metadata4ing#TextVariable"/>
        <rdfs:range rdf:resource="http://www.w3.org/2001/XMLSchema#string"/>
        <rdfs:isDefinedBy rdf:resource="http://w3id.org/nfdi4ing/metadata4ing#"/>
        <skos:prefLabel xml:lang="en">has string value</skos:prefLabel>
        <rdf-syntax-ns:type rdf:resource="https://www.w3.org/2002/07/owl#DatatypeProperty"/>
    </DatatypeProperty>
    


    <!-- http://w3id.org/nfdi4ing/metadata4ing#hasVariableDescription -->


    <DatatypeProperty rdf:about="http://w3id.org/nfdi4ing/metadata4ing#hasVariableDescription">
        <rdfs:domain rdf:resource="http://www.molmod.info/semantics/pims-ii.ttl#Variable"/>
        <rdfs:range rdf:resource="http://www.w3.org/2001/XMLSchema#string"/>
        <rdfs:isDefinedBy rdf:resource="http://w3id.org/nfdi4ing/metadata4ing#"/>
        <skos:prefLabel xml:lang="en">has variable description</skos:prefLabel>
        <rdf-syntax-ns:type rdf:resource="https://www.w3.org/2002/07/owl#DatatypeProperty"/>
    </DatatypeProperty>
    


    <!-- http://w3id.org/nfdi4ing/metadata4ing#identifier -->


    <DatatypeProperty rdf:about="http://w3id.org/nfdi4ing/metadata4ing#identifier">
        <rdfs:domain rdf:resource="https://www.w3.org/2002/07/owl#Thing"/>
        <rdfs:range rdf:resource="http://www.w3.org/2001/XMLSchema#string"/>
        <skos:prefLabel xml:lang="en">identifier</skos:prefLabel>
        <rdf-syntax-ns:type rdf:resource="https://www.w3.org/2002/07/owl#DatatypeProperty"/>
    </DatatypeProperty>
    


    <!-- http://w3id.org/nfdi4ing/metadata4ing#orcidId -->


    <DatatypeProperty rdf:about="http://w3id.org/nfdi4ing/metadata4ing#orcidId">
        <rdfs:subPropertyOf rdf:resource="http://w3id.org/nfdi4ing/metadata4ing#identifier"/>
        <rdfs:domain rdf:resource="http://www.w3.org/ns/prov#Person"/>
        <rdfs:range rdf:resource="http://www.w3.org/2001/XMLSchema#string"/>
        <skos:prefLabel xml:lang="en">has ORCID ID</skos:prefLabel>
        <rdf-syntax-ns:type rdf:resource="https://www.w3.org/2002/07/owl#DatatypeProperty"/>
    </DatatypeProperty>
    


    <!-- http://w3id.org/nfdi4ing/metadata4ing#projectReferenceID -->


    <DatatypeProperty rdf:about="http://w3id.org/nfdi4ing/metadata4ing#projectReferenceID">
        <rdfs:subPropertyOf rdf:resource="http://w3id.org/nfdi4ing/metadata4ing#identifier"/>
        <rdfs:domain rdf:resource="https://schema.org/Project"/>
        <rdfs:range rdf:resource="http://www.w3.org/2001/XMLSchema#string"/>
        <skos:definition xml:lang="en">An alphanumeric identifier for a project.</skos:definition>
        <skos:prefLabel xml:lang="en">has project ID</skos:prefLabel>
        <rdf-syntax-ns:type rdf:resource="https://www.w3.org/2002/07/owl#DatatypeProperty"/>
    </DatatypeProperty>
    


    <!-- http://www.w3.org/ns/dcat#keyword -->


    <DatatypeProperty rdf:about="http://www.w3.org/ns/dcat#keyword">
        <rdfs:domain rdf:resource="http://www.w3.org/ns/dcat#Dataset"/>
        <rdfs:range rdf:resource="http://www.w3.org/2000/01/rdf-schema#Literal"/>
        <skos:definition xml:lang="en">A keyword or tag describing the resource.</skos:definition>
        <skos:prefLabel xml:lang="en">keyword</skos:prefLabel>
        <rdf-syntax-ns:type rdf:resource="https://www.w3.org/2002/07/owl#DatatypeProperty"/>
    </DatatypeProperty>
    


    <!-- http://xmlns.com/foaf/0.1/mbox -->


    <DatatypeProperty rdf:about="http://xmlns.com/foaf/0.1/mbox">
        <rdfs:domain rdf:resource="http://www.w3.org/ns/prov#Agent"/>
        <rdfs:range rdf:resource="https://www.w3.org/2002/07/owl#Thing"/>
        <rdfs:isDefinedBy rdf:resource="http://xmlns.com/foaf/0.1/"/>
        <skos:definition xml:lang="en">A personal mailbox, ie. an Internet mailbox associated with exactly one owner.</skos:definition>
        <skos:prefLabel xml:lang="en">mbox</skos:prefLabel>
        <rdf-syntax-ns:type rdf:resource="https://www.w3.org/2002/07/owl#InverseFunctionalProperty"/>
        <rdf-syntax-ns:type rdf:resource="https://www.w3.org/2002/07/owl#ObjectProperty"/>
    </DatatypeProperty>
    


    <!-- https://matthiasprobst.github.io/ssno#altersUnit -->


    <DatatypeProperty rdf:about="https://matthiasprobst.github.io/ssno#altersUnit">
        <rdfs:domain rdf:resource="https://matthiasprobst.github.io/ssno#Transformation"/>
        <rdfs:range rdf:resource="http://www.w3.org/2001/XMLSchema#string"/>
        <skos:definition xml:lang="en">A string defining how the new unit is generated.</skos:definition>
        <skos:example xml:lang="en">&quot;[X] s-1&quot; where [X] is the unit of the standard name X.</skos:example>
        <skos:prefLabel xml:lang="en">alters unit</skos:prefLabel>
        <rdf-syntax-ns:type rdf:resource="https://www.w3.org/2002/07/owl#DatatypeProperty"/>
    </DatatypeProperty>
    


    <!-- https://matthiasprobst.github.io/ssno#ancillaryVariables -->


    <DatatypeProperty rdf:about="https://matthiasprobst.github.io/ssno#ancillaryVariables">
        <rdfs:domain rdf:resource="http://purl.allotrope.org/ontologies/hdf5/1.8#Dataset"/>
        <rdfs:range rdf:resource="http://www.w3.org/2001/XMLSchema#string"/>
        <skos:definition xml:lang="en">Used to provide metadata about the data the property is provided with. E.g. uncertainties can be expressed/linked like this. As stated in the cf-conventions, the &quot;nature of the relationship between variables associated via ancillary_variables must be determined by other attributes&quot; https://cfconventions.org/Data/cf-conventions/cf-conventions-1.7/build/ch03s04.html)</skos:definition>
        <skos:prefLabel xml:lang="en">ancillary variables</skos:prefLabel>
        <rdf-syntax-ns:type rdf:resource="https://www.w3.org/2002/07/owl#DatatypeProperty"/>
    </DatatypeProperty>
    


    <!-- https://matthiasprobst.github.io/ssno#character -->


    <DatatypeProperty rdf:about="https://matthiasprobst.github.io/ssno#character">
        <rdfs:domain rdf:resource="https://matthiasprobst.github.io/ssno#Character"/>
        <rdfs:range rdf:resource="http://www.w3.org/2001/XMLSchema#string"/>
        <skos:definition xml:lang="en">A character i.e. a single letter or symbol</skos:definition>
        <skos:prefLabel xml:lang="en">character</skos:prefLabel>
        <rdf-syntax-ns:type rdf:resource="https://www.w3.org/2002/07/owl#DatatypeProperty"/>
    </DatatypeProperty>
    


    <!-- https://matthiasprobst.github.io/ssno#hasPreposition -->


    <DatatypeProperty rdf:about="https://matthiasprobst.github.io/ssno#hasPreposition">
        <rdfs:domain rdf:resource="https://matthiasprobst.github.io/ssno#Qualification"/>
        <rdfs:range rdf:resource="http://www.w3.org/2001/XMLSchema#string"/>
        <skos:definition xml:lang="en">A data property that stores prepositional qualifiers like &quot;at,&quot; &quot;in,&quot; &quot;due to,&quot; and &quot;assuming.&quot; to be used with Qualifications.</skos:definition>
        <skos:example xml:lang="en">The CF Convention uses the qualification &apos;in process&apos; where &apos;in&apos; is the preposition and &apos;process&apos; the qualificaiton.</skos:example>
        <skos:prefLabel xml:lang="en">has preposition</skos:prefLabel>
        <rdf-syntax-ns:type rdf:resource="https://www.w3.org/2002/07/owl#DatatypeProperty"/>
    </DatatypeProperty>
    


    <!-- https://matthiasprobst.github.io/ssno#longName -->


    <DatatypeProperty rdf:about="https://matthiasprobst.github.io/ssno#longName">
        <rdfs:domain rdf:resource="http://purl.allotrope.org/ontologies/hdf5/1.8#Dataset"/>
        <rdfs:range rdf:resource="http://www.w3.org/2001/XMLSchema#string"/>
        <skos:definition xml:lang="en">A human-readable label of a variable which is should be used in addition with a standard_name. As intended in the cf-conventions (https://cfconventions.org/Data/cf-conventions/cf-conventions-1.7/build/ch03s02.html), it may be used for labeling plots.</skos:definition>
        <skos:prefLabel xml:lang="en">long name</skos:prefLabel>
        <rdf-syntax-ns:type rdf:resource="https://www.w3.org/2002/07/owl#DatatypeProperty"/>
    </DatatypeProperty>
    


    <!-- https://matthiasprobst.github.io/ssno#standardName -->


    <DatatypeProperty rdf:about="https://matthiasprobst.github.io/ssno#standardName">
        <rdfs:domain rdf:resource="http://org.semanticweb.owlapi/error#Error12"/>
        <rdfs:range rdf:resource="http://www.w3.org/2001/XMLSchema#string"/>
        <rdfs:comment xml:lang="en">If ssno:standardName is associated with an HDF5 Dataset then the corresponding standard name table must be assigned to the root group in order to elaborate the properties of the ssno:StandardName.</rdfs:comment>
        <skos:definition xml:lang="en">Name for a standard name, e.g. &quot;x_velocity&quot;. The construction of a standard name string is defined by the standard name table. E.g. no spaces are allowed and specific pre- and suffixes are allowed.</skos:definition>
        <skos:example xml:lang="en">x_velocity</skos:example>
        <skos:prefLabel xml:lang="en">standard name</skos:prefLabel>
        <rdf-syntax-ns:type rdf:resource="https://www.w3.org/2002/07/owl#DatatypeProperty"/>
    </DatatypeProperty>
    


    <!-- https://matthiasprobst.github.io/ssno#standardNameCharacter -->


    <DatatypeProperty rdf:about="https://matthiasprobst.github.io/ssno#standardNameCharacter">
        <rdfs:domain rdf:resource="https://matthiasprobst.github.io/ssno#Transformation"/>
        <rdfs:range rdf:resource="http://www.w3.org/2001/XMLSchema#string"/>
        <skos:definition xml:lang="en">The character whcih is used in a standard name transformation string to indivate the position a standard name used in the modification rule.</skos:definition>
        <skos:example xml:lang="en">in the transformation string &quot;integral_of_Y_wrt_X&quot; the standard name representation characters are be &quot;X&quot; and &quot;Y&quot;</skos:example>
        <skos:prefLabel xml:lang="en">standard name character</skos:prefLabel>
        <rdf-syntax-ns:type rdf:resource="https://www.w3.org/2002/07/owl#DatatypeProperty"/>
    </DatatypeProperty>
    


    <!-- https://schema.org/name -->


    <DatatypeProperty rdf:about="https://schema.org/name">
        <rdfs:domain rdf:resource="https://matthiasprobst.github.io/ssno#StandardNameModification"/>
        <rdfs:range rdf:resource="http://www.w3.org/2001/XMLSchema#string"/>
        <skos:definition xml:lang="en">The name of the item.</skos:definition>
        <skos:prefLabel xml:lang="en">name</skos:prefLabel>
        <rdf-syntax-ns:type rdf:resource="https://www.w3.org/2002/07/owl#DatatypeProperty"/>
    </DatatypeProperty>
    


    <!-- 
    ///////////////////////////////////////////////////////////////////////////////////////
    //
    // Classes
    //
    ///////////////////////////////////////////////////////////////////////////////////////
     -->


    


    <!-- http://org.semanticweb.owlapi/error#Error1 -->


    <Class rdf:about="http://org.semanticweb.owlapi/error#Error1"/>
    


    <!-- http://org.semanticweb.owlapi/error#Error10 -->


    <Class rdf:about="http://org.semanticweb.owlapi/error#Error10"/>
    


    <!-- http://org.semanticweb.owlapi/error#Error11 -->


    <Class rdf:about="http://org.semanticweb.owlapi/error#Error11"/>
    


    <!-- http://org.semanticweb.owlapi/error#Error12 -->


    <Class rdf:about="http://org.semanticweb.owlapi/error#Error12"/>
    


    <!-- http://org.semanticweb.owlapi/error#Error13 -->


    <Class rdf:about="http://org.semanticweb.owlapi/error#Error13"/>
    


    <!-- http://org.semanticweb.owlapi/error#Error14 -->


    <Class rdf:about="http://org.semanticweb.owlapi/error#Error14"/>
    


    <!-- http://org.semanticweb.owlapi/error#Error15 -->


    <Class rdf:about="http://org.semanticweb.owlapi/error#Error15"/>
    


    <!-- http://org.semanticweb.owlapi/error#Error16 -->


    <Class rdf:about="http://org.semanticweb.owlapi/error#Error16"/>
    


    <!-- http://org.semanticweb.owlapi/error#Error17 -->


    <Class rdf:about="http://org.semanticweb.owlapi/error#Error17"/>
    


    <!-- http://org.semanticweb.owlapi/error#Error18 -->


    <Class rdf:about="http://org.semanticweb.owlapi/error#Error18"/>
    


    <!-- http://org.semanticweb.owlapi/error#Error19 -->


    <Class rdf:about="http://org.semanticweb.owlapi/error#Error19"/>
    


    <!-- http://org.semanticweb.owlapi/error#Error2 -->


    <Class rdf:about="http://org.semanticweb.owlapi/error#Error2"/>
    


    <!-- http://org.semanticweb.owlapi/error#Error20 -->


    <Class rdf:about="http://org.semanticweb.owlapi/error#Error20"/>
    


    <!-- http://org.semanticweb.owlapi/error#Error21 -->


    <Class rdf:about="http://org.semanticweb.owlapi/error#Error21"/>
    


    <!-- http://org.semanticweb.owlapi/error#Error3 -->


    <Class rdf:about="http://org.semanticweb.owlapi/error#Error3"/>
    


    <!-- http://org.semanticweb.owlapi/error#Error4 -->


    <Class rdf:about="http://org.semanticweb.owlapi/error#Error4"/>
    


    <!-- http://org.semanticweb.owlapi/error#Error5 -->


    <Class rdf:about="http://org.semanticweb.owlapi/error#Error5"/>
    


    <!-- http://org.semanticweb.owlapi/error#Error6 -->


    <Class rdf:about="http://org.semanticweb.owlapi/error#Error6"/>
    


    <!-- http://org.semanticweb.owlapi/error#Error8 -->


    <Class rdf:about="http://org.semanticweb.owlapi/error#Error8"/>
    


    <!-- http://org.semanticweb.owlapi/error#Error9 -->


    <Class rdf:about="http://org.semanticweb.owlapi/error#Error9"/>
    


    <!-- http://purl.allotrope.org/ontologies/hdf5/1.8#Dataset -->


    <Class rdf:about="http://purl.allotrope.org/ontologies/hdf5/1.8#Dataset">
        <rdfs:isDefinedBy rdf:resource="http://purl.allotrope.org/ontologies/hdf5/1.8#"/>
        <skos:definition xml:lang="en">An HDF5 Dataset.</skos:definition>
        <skos:prefLabel xml:lang="en">HDF5 Dataset</skos:prefLabel>
        <rdf-syntax-ns:type rdf:resource="https://www.w3.org/2002/07/owl#Class"/>
    </Class>
    


    <!-- http://purl.allotrope.org/ontologies/hdf5/1.8#Group -->


    <Class rdf:about="http://purl.allotrope.org/ontologies/hdf5/1.8#Group">
        <rdfs:isDefinedBy rdf:resource="http://purl.allotrope.org/ontologies/hdf5/1.8#"/>
        <skos:definition xml:lang="en">A grouping structure containing instances of zero or more groups or datasets, together with supporting metadata.</skos:definition>
        <skos:prefLabel xml:lang="en">HDF5 Group</skos:prefLabel>
        <rdf-syntax-ns:type rdf:resource="https://www.w3.org/2002/07/owl#Class"/>
    </Class>
    


    <!-- http://qudt.org/schema/qudt/Unit -->


    <Class rdf:about="http://qudt.org/schema/qudt/Unit">
        <skos:definition xml:lang="en">Unit of measure.</skos:definition>
        <skos:prefLabel xml:lang="en">Unit</skos:prefLabel>
        <rdf-syntax-ns:type rdf:resource="https://www.w3.org/2002/07/owl#Class"/>
    </Class>
    


    <!-- http://w3id.org/nfdi4ing/metadata4ing#NumericalVariable -->


    <Class rdf:about="http://w3id.org/nfdi4ing/metadata4ing#NumericalVariable">
        <rdfs:subClassOf rdf:resource="http://www.molmod.info/semantics/pims-ii.ttl#Variable"/>
        <rdfs:isDefinedBy rdf:resource="http://w3id.org/nfdi4ing/metadata4ing#"/>
        <skos:closeMatch rdf:resource="https://ptb.de/si/Real"/>
        <skos:definition xml:lang="en">A variable that expects a float or integer as a value</skos:definition>
        <skos:prefLabel xml:lang="en">numerical variable</skos:prefLabel>
        <rdf-syntax-ns:type rdf:resource="https://www.w3.org/2002/07/owl#Class"/>
    </Class>
    


    <!-- http://w3id.org/nfdi4ing/metadata4ing#TextVariable -->


    <Class rdf:about="http://w3id.org/nfdi4ing/metadata4ing#TextVariable">
        <rdfs:subClassOf rdf:resource="http://www.molmod.info/semantics/pims-ii.ttl#Variable"/>
        <rdfs:isDefinedBy rdf:resource="http://w3id.org/nfdi4ing/metadata4ing#"/>
        <skos:prefLabel xml:lang="en">text variable</skos:prefLabel>
        <rdf-syntax-ns:type rdf:resource="https://www.w3.org/2002/07/owl#Class"/>
    </Class>
    


    <!-- http://www.molmod.info/semantics/pims-ii.ttl#Property -->


    <Class rdf:about="http://www.molmod.info/semantics/pims-ii.ttl#Property">
        <rdfs:subClassOf rdf:resource="http://www.molmod.info/semantics/pims-ii.ttl#Variable"/>
        <skos:closeMatch rdf:resource="https://emmo.info/emmo#EMMO_b7bcff25_ffc3_474e_9ab5_01b1664bd4ba"/>
        <skos:definition xml:lang="en">Property, i.e., a variable that can be considered (as an investigated property, i.e., target property) within a processing step</skos:definition>
        <skos:prefLabel xml:lang="en">Property</skos:prefLabel>
        <rdf-syntax-ns:type rdf:resource="https://www.w3.org/2002/07/owl#Class"/>
    </Class>
    


    <!-- http://www.molmod.info/semantics/pims-ii.ttl#QuantityValue -->


    <Class rdf:about="http://www.molmod.info/semantics/pims-ii.ttl#QuantityValue">
        <rdfs:subClassOf rdf:resource="https://schema.org/Intangible"/>
        <rdfs:isDefinedBy rdf:resource="http://www.molmod.info/semantics/pims-ii.ttl#"/>
        <skos:definition xml:lang="en">Quantity value, i.e., a value that has a numerical magnitude and a physical unit</skos:definition>
        <skos:prefLabel xml:lang="en">quantity value</skos:prefLabel>
        <rdf-syntax-ns:type rdf:resource="https://www.w3.org/2002/07/owl#Class"/>
    </Class>
    


    <!-- http://www.molmod.info/semantics/pims-ii.ttl#Variable -->


    <Class rdf:about="http://www.molmod.info/semantics/pims-ii.ttl#Variable">
        <rdfs:subClassOf rdf:resource="https://schema.org/Intangible"/>
        <skos:definition xml:lang="en">Variable, i.e., a conventional that is employed for something to which values can be assigned (this may include different notations for the same variable including, e.g., computational representations); this is to be understood very generally, e.g., a variable may be an array or set of elements or have another kind of internal structure</skos:definition>
        <skos:prefLabel xml:lang="en">Variable</skos:prefLabel>
        <rdf-syntax-ns:type rdf:resource="https://www.w3.org/2002/07/owl#Class"/>
    </Class>
    


    <!-- http://www.w3.org/2004/02/skos/core#Concept -->


    <Class rdf:about="http://www.w3.org/2004/02/skos/core#Concept">
        <skos:definition xml:lang="en">A SKOS concept can be viewed as an idea or notion; a unit of thought. However, what constitutes a unit of thought is subjective, and this definition is meant to be suggestive, rather than restrictive.</skos:definition>
        <skos:prefLabel xml:lang="en">Concept</skos:prefLabel>
        <rdf-syntax-ns:type rdf:resource="https://www.w3.org/2002/07/owl#Class"/>
    </Class>
    


    <!-- http://www.w3.org/ns/dcat#Dataset -->


    <Class rdf:about="http://www.w3.org/ns/dcat#Dataset">
        <rdfs:isDefinedBy rdf:resource="http://www.w3.org/ns/dcat#"/>
        <skos:definition xml:lang="en">A collection of data, published or curated by a single agent, and available for access or download in one or more representations.</skos:definition>
        <skos:prefLabel xml:lang="en">Dataset</skos:prefLabel>
        <rdf-syntax-ns:type rdf:resource="https://www.w3.org/2002/07/owl#Class"/>
        <owl1:equivalentClass rdf:nodeID="genid2"/>
    </Class>
    <rdf:Description rdf:nodeID="genid2">
        <rdf-syntax-ns:type rdf:resource="https://www.w3.org/2002/07/owl#Restriction"/>
        <owl1:onProperty>
            <rdf:Description>
                <owl1:inverseOf rdf:resource="https://matthiasprobst.github.io/ssno#standardNameTableUsedBy"/>
            </rdf:Description>
        </owl1:onProperty>
        <owl1:someValuesFrom rdf:resource="https://matthiasprobst.github.io/ssno#StandardNameTable"/>
    </rdf:Description>
    


    <!-- http://www.w3.org/ns/dcat#Role -->


    <Class rdf:about="http://www.w3.org/ns/dcat#Role">
        <rdfs:subClassOf rdf:resource="http://www.w3.org/2004/02/skos/core#Concept"/>
        <rdfs:comment xml:lang="en">Used in a qualified-attribution to specify the role of an Agent with respect to an Entity. It is recommended that the values be managed as a controlled vocabulary of agent roles, such as ISO-19115-1 CI_RoleCode (https://standards.iso.org/iso/19115/resources/Codelists/gml/CI_RoleCode.xml)</rdfs:comment>
        <skos:definition xml:lang="en">A role is the function of a resource or agent with respect to another resource, in the context of resource attribution or resource relationships.</skos:definition>
        <skos:prefLabel xml:lang="en">Role</skos:prefLabel>
        <rdf-syntax-ns:type rdf:resource="https://www.w3.org/2002/07/owl#Class"/>
    </Class>
    


    <!-- http://www.w3.org/ns/prov#Agent -->


    <Class rdf:about="http://www.w3.org/ns/prov#Agent">
        <rdfs:isDefinedBy rdf:resource="http://www.w3.org/ns/prov#"/>
        <skos:definition xml:lang="en">Person or Organization related to a StandardNameTable.</skos:definition>
        <skos:prefLabel xml:lang="en">Agent</skos:prefLabel>
        <rdf-syntax-ns:type rdf:resource="https://www.w3.org/2002/07/owl#Class"/>
    </Class>
    


    <!-- http://www.w3.org/ns/prov#Attribution -->


    <Class rdf:about="http://www.w3.org/ns/prov#Attribution">
        <skos:definition xml:lang="en">Attribution is the ascribing of an entity to an agent. When an entity e is attributed to agent ag, entity e was generated by some unspecified activity that in turn was associated to agent ag. Thus, this relation is useful when the activity is not known, or irrelevant.</skos:definition>
        <skos:prefLabel xml:lang="en">Attribution</skos:prefLabel>
        <rdf-syntax-ns:type rdf:resource="https://www.w3.org/2002/07/owl#Class"/>
    </Class>
    


    <!-- http://www.w3.org/ns/prov#Organization -->


    <Class rdf:about="http://www.w3.org/ns/prov#Organization">
        <rdfs:subClassOf rdf:resource="http://www.w3.org/ns/prov#Agent"/>
        <skos:prefLabel xml:lang="en">Organization</skos:prefLabel>
        <rdf-syntax-ns:type rdf:resource="https://www.w3.org/2002/07/owl#Class"/>
    </Class>
    


    <!-- http://www.w3.org/ns/prov#Person -->


    <Class rdf:about="http://www.w3.org/ns/prov#Person">
        <rdfs:subClassOf rdf:resource="http://www.w3.org/ns/prov#Agent"/>
        <skos:prefLabel xml:lang="en">Person</skos:prefLabel>
        <rdf-syntax-ns:type rdf:resource="https://www.w3.org/2002/07/owl#Class"/>
    </Class>
    


    <!-- https://matthiasprobst.github.io/ssno#Character -->


    <Class rdf:about="https://matthiasprobst.github.io/ssno#Character">
        <skos:prefLabel xml:lang="en">Charakter</skos:prefLabel>
        <rdf-syntax-ns:type rdf:resource="https://www.w3.org/2002/07/owl#Class"/>
    </Class>
    


    <!-- https://matthiasprobst.github.io/ssno#Qualification -->


    <Class rdf:about="https://matthiasprobst.github.io/ssno#Qualification">
        <rdfs:subClassOf rdf:resource="http://org.semanticweb.owlapi/error#Error14"/>
        <rdfs:subClassOf rdf:resource="https://matthiasprobst.github.io/ssno#StandardNameModification"/>
        <skos:definition xml:lang="en">A qualification derives an existing standard name by a rule. This may alter the units.</skos:definition>
        <skos:example xml:lang="en">See here https://cfconventions.org/Data/cf-standard-names/docs/guidelines.html</skos:example>
        <skos:prefLabel xml:lang="en">Qualification</skos:prefLabel>
        <rdf-syntax-ns:type rdf:resource="https://www.w3.org/2002/07/owl#Class"/>
        <owl1:disjointWith rdf:resource="https://matthiasprobst.github.io/ssno#Transformation"/>
    </Class>
    


    <!-- https://matthiasprobst.github.io/ssno#ScalarStandardName -->


    <Class rdf:about="https://matthiasprobst.github.io/ssno#ScalarStandardName">
        <rdfs:subClassOf rdf:resource="https://matthiasprobst.github.io/ssno#StandardName"/>
        <skos:definition xml:lang="en">A standard name associated with scalar data.</skos:definition>
        <skos:prefLabel xml:lang="en">Scalar Standard Name</skos:prefLabel>
        <rdf-syntax-ns:type rdf:resource="https://www.w3.org/2002/07/owl#Class"/>
        <owl1:disjointWith rdf:resource="https://matthiasprobst.github.io/ssno#VectorStandardName"/>
    </Class>
    


    <!-- https://matthiasprobst.github.io/ssno#StandardName -->


    <Class rdf:about="https://matthiasprobst.github.io/ssno#StandardName">
        <rdfs:subClassOf rdf:resource="http://org.semanticweb.owlapi/error#Error20"/>
        <skos:definition xml:lang="en">A standard name is defined by a canonical unit and a description. It generally is defined by a standard name table.</skos:definition>
        <skos:prefLabel xml:lang="en">Standard Name</skos:prefLabel>
        <rdf-syntax-ns:type rdf:resource="https://www.w3.org/2002/07/owl#Class"/>
        <owl1:equivalentClass rdf:nodeID="genid4"/>
    </Class>
    <rdf:Description rdf:nodeID="genid4">
        <rdf-syntax-ns:type rdf:resource="https://www.w3.org/2002/07/owl#Restriction"/>
        <owl1:onProperty>
            <rdf:Description>
                <owl1:inverseOf rdf:resource="https://matthiasprobst.github.io/ssno#standardNames"/>
            </rdf:Description>
        </owl1:onProperty>
        <owl1:someValuesFrom rdf:resource="https://matthiasprobst.github.io/ssno#StandardNameTable"/>
    </rdf:Description>
    


    <!-- https://matthiasprobst.github.io/ssno#StandardNameModification -->


    <Class rdf:about="https://matthiasprobst.github.io/ssno#StandardNameModification">
        <skos:definition xml:lang="en">A concept which defines the construction of a standard name, e.g. by adding specific phrases following well-defined rules. It extends or changes a base standard name and hence may or may not change the unit of it.</skos:definition>
        <skos:prefLabel xml:lang="en">Standard Name Modification</skos:prefLabel>
        <rdf-syntax-ns:type rdf:resource="https://www.w3.org/2002/07/owl#Class"/>
    </Class>
    


    <!-- https://matthiasprobst.github.io/ssno#StandardNameTable -->


    <Class rdf:about="https://matthiasprobst.github.io/ssno#StandardNameTable">
        <rdfs:subClassOf rdf:resource="http://org.semanticweb.owlapi/error#Error15"/>
        <rdfs:subClassOf rdf:resource="http://org.semanticweb.owlapi/error#Error16"/>
        <rdfs:subClassOf rdf:resource="http://org.semanticweb.owlapi/error#Error17"/>
        <rdfs:subClassOf rdf:resource="http://www.w3.org/2004/02/skos/core#Concept"/>
        <skos:definition xml:lang="en">A standard name table holds a list of all available standard names used in a certain context (project, domain, ...) and gives further information about version and contact.</skos:definition>
        <skos:prefLabel xml:lang="en">Standard NameTable</skos:prefLabel>
        <rdf-syntax-ns:type rdf:resource="https://www.w3.org/2002/07/owl#Class"/>
        <owl1:equivalentClass rdf:nodeID="genid6"/>
        <owl1:equivalentClass rdf:nodeID="genid8"/>
        <owl1:equivalentClass rdf:nodeID="genid10"/>
    </Class>
    <rdf:Description rdf:nodeID="genid6">
        <rdf-syntax-ns:type rdf:resource="https://www.w3.org/2002/07/owl#Restriction"/>
        <owl1:onProperty>
            <rdf:Description>
                <owl1:inverseOf rdf:resource="https://matthiasprobst.github.io/ssno#standardNameTable"/>
            </rdf:Description>
        </owl1:onProperty>
        <owl1:someValuesFrom rdf:resource="https://matthiasprobst.github.io/ssno#StandardName"/>
    </rdf:Description>
    <rdf:Description rdf:nodeID="genid8">
        <rdf-syntax-ns:type rdf:resource="https://www.w3.org/2002/07/owl#Restriction"/>
        <owl1:onProperty>
            <rdf:Description>
                <owl1:inverseOf rdf:resource="https://matthiasprobst.github.io/ssno#usesStandardNameTable"/>
            </rdf:Description>
        </owl1:onProperty>
        <owl1:someValuesFrom rdf:resource="http://purl.allotrope.org/ontologies/hdf5/1.8#File"/>
    </rdf:Description>
    <rdf:Description rdf:nodeID="genid10">
        <rdf-syntax-ns:type rdf:resource="https://www.w3.org/2002/07/owl#Restriction"/>
        <owl1:onProperty>
            <rdf:Description>
                <owl1:inverseOf rdf:resource="https://matthiasprobst.github.io/ssno#usesStandardNameTable"/>
            </rdf:Description>
        </owl1:onProperty>
        <owl1:someValuesFrom rdf:resource="http://www.w3.org/ns/dcat#Dataset"/>
    </rdf:Description>
    


    <!-- https://matthiasprobst.github.io/ssno#Transformation -->


    <Class rdf:about="https://matthiasprobst.github.io/ssno#Transformation">
        <rdfs:subClassOf rdf:resource="http://org.semanticweb.owlapi/error#Error19"/>
        <rdfs:subClassOf rdf:resource="https://matthiasprobst.github.io/ssno#StandardNameModification"/>
        <skos:definition xml:lang="en">A transfromation is a phrase which may be added to the standard name without changing its unit.</skos:definition>
        <skos:prefLabel xml:lang="en">Transformation</skos:prefLabel>
        <rdf-syntax-ns:type rdf:resource="https://www.w3.org/2002/07/owl#Class"/>
    </Class>
    


    <!-- https://matthiasprobst.github.io/ssno#VectorQualification -->


    <Class rdf:about="https://matthiasprobst.github.io/ssno#VectorQualification">
        <rdfs:subClassOf rdf:resource="https://matthiasprobst.github.io/ssno#Qualification"/>
        <rdfs:comment xml:lang="en">A vector component qualification holding values like &quot;x&quot;, &quot;y&quot; and &quot;z&quot; can modify vector standard names like &quot;velocity&quot; but not scalar standard names like &quot;pressure&quot;.</rdfs:comment>
        <skos:definition xml:lang="en">Special Qualification accounting for Vector Standard Names. Only one such Qualification must exist at max in a StandardNameTable</skos:definition>
        <skos:prefLabel xml:lang="en">Vector Qualification</skos:prefLabel>
        <rdf-syntax-ns:type rdf:resource="https://www.w3.org/2002/07/owl#Class"/>
    </Class>
    


    <!-- https://matthiasprobst.github.io/ssno#VectorStandardName -->


    <Class rdf:about="https://matthiasprobst.github.io/ssno#VectorStandardName">
        <rdfs:subClassOf rdf:resource="https://matthiasprobst.github.io/ssno#StandardName"/>
        <skos:definition xml:lang="en">A standard name associated with vector data.</skos:definition>
        <skos:prefLabel xml:lang="en">Vector Standard Name</skos:prefLabel>
        <rdf-syntax-ns:type rdf:resource="https://www.w3.org/2002/07/owl#Class"/>
    </Class>
    


    <!-- https://schema.org/Intangible -->


    <Class rdf:about="https://schema.org/Intangible">
        <skos:definition xml:lang="en">A utility class that serves as the umbrella for a number of &apos;intangible&apos; things such as quantities, structured values, etc.</skos:definition>
        <skos:prefLabel xml:lang="en">Intangible</skos:prefLabel>
        <rdf-syntax-ns:type rdf:resource="https://www.w3.org/2002/07/owl#Class"/>
    </Class>
    


    <!-- https://schema.org/Project -->


    <Class rdf:about="https://schema.org/Project">
        <rdfs:comment xml:lang="en">An enterprise (potentially individual but typically collaborative), planned to achieve a particular aim</rdfs:comment>
        <skos:prefLabel xml:lang="en">Project</skos:prefLabel>
        <rdf-syntax-ns:type rdf:resource="https://www.w3.org/2002/07/owl#Class"/>
    </Class>
    


    <!-- https://schema.org/ResearchProject -->


    <Class rdf:about="https://schema.org/ResearchProject">
        <rdfs:subClassOf rdf:resource="https://schema.org/Project"/>
        <skos:definition xml:lang="en">A Research project.</skos:definition>
        <skos:prefLabel xml:lang="en">Research Project</skos:prefLabel>
        <rdf-syntax-ns:type rdf:resource="https://www.w3.org/2002/07/owl#Class"/>
    </Class>
    


    <!-- 
    ///////////////////////////////////////////////////////////////////////////////////////
    //
    // Individuals
    //
    ///////////////////////////////////////////////////////////////////////////////////////
     -->


    


    <!-- https://matthiasprobst.github.io/ssno# -->


    <NamedIndividual rdf:about="https://matthiasprobst.github.io/ssno#">
        <terms:title xml:lang="en">sSNO: A simple Standard Name Ontology</terms:title>
        <terms:abstract xml:lang="en">This is an ontology draft for the usage of standard names as a simple way of describing complex data. It is motivated by the [cf-conventions](https://cfconventions.org/), which introduced the concept of standard names originally. However, SSNO may (at this stage) not cover all aspects of the original, therefore it is called &quot;simple&quot;. With this ontology, its usage shall be applicable to other research topics, too. The core idea is to provide the class StandardName and StandardNameTable with a minimal set of properties. The rules of standard name construction is defined in a document associated with the standard name table. The table contains all standard names defied by a project or community. Instances of StandardName and StandardNameTable can be used e.g. in combinations with other ontologies like [metadata4ing](https://nfdi4ing.pages.rwth-aachen.de/metadata4ing/metadata4ing/) for a concise description of a numerical variable.</terms:abstract>
        <terms:created>2024-01-15</terms:created>
        <terms:creator>Matthias Probst (https://orcid.org/0000-0001-8729-0482), Institut für Thermische Strömungsmaschinen</terms:creator>
        <terms:license rdf:resource="https://creativecommons.org/licenses/by/4.0/"/>
        <terms:rights rdf:resource="https://creativecommons.org/licenses/by/4.0/"/>
        <vann:preferredNamespacePrefix>ssno</vann:preferredNamespacePrefix>
        <vann:preferredNamespaceUri>https://matthiasprobst.github.io/ssno#</vann:preferredNamespaceUri>
        <rdfs:label>sSNO</rdfs:label>
        <rdf-syntax-ns:type rdf:resource="https://www.w3.org/2002/07/owl#Ontology"/>
        <owl1:versionIRI rdf:resource="https://matthiasprobst.github.io/ssno/1.3.0"/>
        <owl1:versionInfo>v1.3.0</owl1:versionInfo>
    </NamedIndividual>
    


    <!-- https://matthiasprobst.github.io/ssno#AnyStandardName -->


    <NamedIndividual rdf:about="https://matthiasprobst.github.io/ssno#AnyStandardName">
        <ssno:unit rdf:resource="https://matthiasprobst.github.io/ssno#AnyUnit"/>
        <skos:prefLabel xml:lang="en">Any Standard Name</skos:prefLabel>
        <ssno:description xml:lang="en">A generic Standard Name. Intended to be used to refer to any Standard Name, e.g. by relating the position of a qualification to it, i.e. to be placed before or after a Standard Name.</ssno:description>
        <ssno:description xml:lang="de">Ein generischer Standardname um Qualifications in Relation zu setzen.</ssno:description>
        <rdf-syntax-ns:type rdf:resource="https://matthiasprobst.github.io/ssno#StandardName"/>
        <rdf-syntax-ns:type rdf:resource="https://www.w3.org/2002/07/owl#NamedIndividual"/>
    </NamedIndividual>
    


    <!-- https://matthiasprobst.github.io/ssno#AnyUnit -->


    <NamedIndividual rdf:about="https://matthiasprobst.github.io/ssno#AnyUnit">
        <skos:definition xml:lang="en">Representing any physical unit.</skos:definition>
        <skos:prefLabel xml:lang="en">any unit</skos:prefLabel>
        <rdf-syntax-ns:type rdf:resource="http://qudt.org/schema/qudt/Unit"/>
        <rdf-syntax-ns:type rdf:resource="https://www.w3.org/2002/07/owl#NamedIndividual"/>
    </NamedIndividual>
    <rdf:Description rdf:nodeID="genid12">
        <rdf-syntax-ns:type rdf:resource="https://www.w3.org/2002/07/owl#Class"/>
        <owl1:unionOf>
            <rdf:Description/>
        </owl1:unionOf>
    </rdf:Description>
    <rdf:Description rdf:nodeID="genid14">
        <rdf-syntax-ns:type rdf:resource="https://www.w3.org/2002/07/owl#Class"/>
        <owl1:unionOf>
            <rdf:Description/>
        </owl1:unionOf>
    </rdf:Description>
    <rdf:Description rdf:nodeID="genid16">
        <rdf-syntax-ns:type rdf:resource="https://www.w3.org/2002/07/owl#Class"/>
        <owl1:unionOf>
            <rdf:Description/>
        </owl1:unionOf>
    </rdf:Description>
    <rdf:Description rdf:nodeID="genid18">
        <rdf-syntax-ns:type rdf:resource="https://www.w3.org/2002/07/owl#Class"/>
        <owl1:unionOf>
            <rdf:Description/>
        </owl1:unionOf>
    </rdf:Description>
    <rdf:Description rdf:nodeID="genid20">
        <rdf-syntax-ns:type rdf:resource="https://www.w3.org/2002/07/owl#Class"/>
        <owl1:unionOf>
            <rdf:Description/>
        </owl1:unionOf>
    </rdf:Description>
    <rdf:Description rdf:nodeID="genid22">
        <rdf-syntax-ns:type rdf:resource="https://www.w3.org/2002/07/owl#Class"/>
        <owl1:unionOf>
            <rdf:Description/>
        </owl1:unionOf>
    </rdf:Description>
    <rdf:Description rdf:nodeID="genid24">
        <rdf-syntax-ns:type rdf:resource="https://www.w3.org/2002/07/owl#Class"/>
        <owl1:unionOf>
            <rdf:Description/>
        </owl1:unionOf>
    </rdf:Description>
    <rdf:Description rdf:nodeID="genid26">
        <rdf-syntax-ns:type rdf:resource="http://www.w3.org/2000/01/rdf-schema#Datatype"/>
        <owl1:unionOf>
            <rdf:Description/>
        </owl1:unionOf>
    </rdf:Description>
    <rdf:Description rdf:nodeID="genid28">
        <rdf-syntax-ns:type rdf:resource="http://www.w3.org/2000/01/rdf-schema#Datatype"/>
        <owl1:onDatatype rdf:resource="http://www.w3.org/2001/XMLSchema#string"/>
        <owl1:withRestrictions>
            <rdf:Description/>
        </owl1:withRestrictions>
    </rdf:Description>
    <rdf:Description rdf:nodeID="genid30">
        <rdf-syntax-ns:type rdf:resource="https://www.w3.org/2002/07/owl#Class"/>
        <owl1:unionOf>
            <rdf:Description/>
        </owl1:unionOf>
    </rdf:Description>
    <rdf:Description rdf:nodeID="genid32">
        <rdf-syntax-ns:type rdf:resource="https://www.w3.org/2002/07/owl#Class"/>
        <owl1:unionOf>
            <rdf:Description/>
        </owl1:unionOf>
    </rdf:Description>
    <rdf:Description rdf:nodeID="genid34">
        <rdf-syntax-ns:type rdf:resource="https://www.w3.org/2002/07/owl#Class"/>
        <owl1:unionOf>
            <rdf:Description/>
        </owl1:unionOf>
    </rdf:Description>
    <rdf:Description rdf:nodeID="genid36">
        <rdf-syntax-ns:type rdf:resource="https://www.w3.org/2002/07/owl#Restriction"/>
        <owl1:maxQualifiedCardinality rdf:datatype="http://www.w3.org/2001/XMLSchema#nonNegativeInteger">1</owl1:maxQualifiedCardinality>
        <owl1:onClass rdf:resource="https://matthiasprobst.github.io/ssno#VectorQualification"/>
        <owl1:onProperty rdf:resource="https://matthiasprobst.github.io/ssno#hasModifier"/>
    </rdf:Description>
    <rdf:Description rdf:nodeID="genid37">
        <rdf-syntax-ns:type rdf:resource="https://www.w3.org/2002/07/owl#Restriction"/>
        <owl1:minQualifiedCardinality rdf:datatype="http://www.w3.org/2001/XMLSchema#nonNegativeInteger">1</owl1:minQualifiedCardinality>
        <owl1:onDataRange rdf:nodeID="genid38"/>
        <owl1:onProperty rdf:resource="https://matthiasprobst.github.io/ssno#description"/>
    </rdf:Description>
    <rdf:Description rdf:nodeID="genid38">
        <rdf-syntax-ns:type rdf:resource="http://www.w3.org/2000/01/rdf-schema#Datatype"/>
        <owl1:unionOf>
            <rdf:Description/>
        </owl1:unionOf>
    </rdf:Description>
    <rdf:Description rdf:nodeID="genid40">
        <rdf-syntax-ns:type rdf:resource="https://www.w3.org/2002/07/owl#Restriction"/>
        <owl1:onClass rdf:resource="http://qudt.org/schema/qudt/Unit"/>
        <owl1:onProperty rdf:resource="https://matthiasprobst.github.io/ssno#unit"/>
        <owl1:qualifiedCardinality rdf:datatype="http://www.w3.org/2001/XMLSchema#nonNegativeInteger">1</owl1:qualifiedCardinality>
    </rdf:Description>
    <rdf:Description rdf:nodeID="genid41">
        <rdf-syntax-ns:type rdf:resource="https://www.w3.org/2002/07/owl#Restriction"/>
        <owl1:minQualifiedCardinality rdf:datatype="http://www.w3.org/2001/XMLSchema#nonNegativeInteger">1</owl1:minQualifiedCardinality>
        <owl1:onDataRange rdf:nodeID="genid42"/>
        <owl1:onProperty rdf:resource="https://matthiasprobst.github.io/ssno#description"/>
    </rdf:Description>
    <rdf:Description rdf:nodeID="genid42">
        <rdf-syntax-ns:type rdf:resource="http://www.w3.org/2000/01/rdf-schema#Datatype"/>
        <owl1:unionOf>
            <rdf:Description/>
        </owl1:unionOf>
    </rdf:Description>
    <rdf:Description rdf:nodeID="genid44">
        <rdf-syntax-ns:type rdf:resource="https://www.w3.org/2002/07/owl#Class"/>
        <owl1:unionOf>
            <rdf:Description/>
        </owl1:unionOf>
    </rdf:Description>
    <rdf:Description rdf:nodeID="genid46">
        <rdf-syntax-ns:type rdf:resource="https://www.w3.org/2002/07/owl#Class"/>
        <owl1:unionOf>
            <rdf:Description/>
        </owl1:unionOf>
    </rdf:Description>
    <rdf:Description rdf:nodeID="genid48">
        <rdf-syntax-ns:type rdf:resource="https://www.w3.org/2002/07/owl#Class"/>
        <owl1:unionOf>
            <rdf:Description/>
        </owl1:unionOf>
    </rdf:Description>
    <rdf:Description rdf:nodeID="genid50">
        <rdf-syntax-ns:type rdf:resource="https://www.w3.org/2002/07/owl#Restriction"/>
        <owl1:minQualifiedCardinality rdf:datatype="http://www.w3.org/2001/XMLSchema#nonNegativeInteger">1</owl1:minQualifiedCardinality>
        <owl1:onDataRange rdf:nodeID="genid51"/>
        <owl1:onProperty rdf:resource="https://matthiasprobst.github.io/ssno#description"/>
    </rdf:Description>
    <rdf:Description rdf:nodeID="genid51">
        <rdf-syntax-ns:type rdf:resource="http://www.w3.org/2000/01/rdf-schema#Datatype"/>
        <owl1:unionOf>
            <rdf:Description/>
        </owl1:unionOf>
    </rdf:Description>
    <rdf:Description rdf:nodeID="genid53">
        <rdf-syntax-ns:type rdf:resource="https://www.w3.org/2002/07/owl#Restriction"/>
        <owl1:cardinality rdf:datatype="http://www.w3.org/2001/XMLSchema#nonNegativeInteger">1</owl1:cardinality>
        <owl1:onProperty rdf:resource="http://purl.org/dc/terms/hasVersion"/>
    </rdf:Description>
    <rdf:Description>
        <xsd:pattern>https://ror.org/[0-9][0-9][a-z0-9][a-z0-9][a-z0-9][a-z0-9][a-z0-9][0-9][0-9]</xsd:pattern>
    </rdf:Description>
    


    <!-- 
    ///////////////////////////////////////////////////////////////////////////////////////
    //
    // Annotations
    //
    ///////////////////////////////////////////////////////////////////////////////////////
     -->


    <rdf:Description rdf:about="http://purl.allotrope.org/ontologies/hdf5/1.8#File">
        <rdfs:isDefinedBy rdf:resource="http://purl.allotrope.org/ontologies/hdf5/1.8#"/>
        <skos:definition xml:lang="en">A container for storing grouped collections of multi-dimensional arrays containing scientific data following the HDF 5 specification</skos:definition>
        <skos:prefLabel xml:lang="en">HDF5 File</skos:prefLabel>
        <rdf-syntax-ns:type rdf:resource="https://www.w3.org/2002/07/owl#Class"/>
    </rdf:Description>
    <rdf:Description rdf:about="http://purl.org/dc/terms/modified">
        <rdf-syntax-ns:type rdf:resource="https://www.w3.org/2002/07/owl#AnnotationProperty"/>
    </rdf:Description>
    <rdf:Description rdf:about="https://matthiasprobst.github.io/ssno#after">
        <skos:definition xml:lang="en">Refers to another qualification to indicate the order. The qualification it points to is ordered before this one. It can also point to a standard name, which means that this qualification is used right after it.</skos:definition>
        <skos:prefLabel xml:lang="en">after</skos:prefLabel>
        <rdf-syntax-ns:type rdf:resource="https://www.w3.org/2002/07/owl#FunctionalProperty"/>
        <rdf-syntax-ns:type rdf:resource="https://www.w3.org/2002/07/owl#ObjectProperty"/>
    </rdf:Description>
    <rdf:Description rdf:about="https://matthiasprobst.github.io/ssno#before">
        <skos:definition xml:lang="en">Refers to another qualification to indicate the order. The qualification it points to is ordered after this one. It can also point to a standard name, which means that this qualification is used right before it.</skos:definition>
        <skos:prefLabel xml:lang="en">before</skos:prefLabel>
        <rdf-syntax-ns:type rdf:resource="https://www.w3.org/2002/07/owl#FunctionalProperty"/>
        <rdf-syntax-ns:type rdf:resource="https://www.w3.org/2002/07/owl#ObjectProperty"/>
    </rdf:Description>
    <rdf:Description rdf:about="https://matthiasprobst.github.io/ssno#description">
        <skos:definition xml:lang="en">Description of a Standard Name, a qualification or a transformation.</skos:definition>
        <skos:prefLabel xml:lang="en">description</skos:prefLabel>
        <rdf-syntax-ns:type rdf:resource="https://www.w3.org/2002/07/owl#DatatypeProperty"/>
    </rdf:Description>
    <rdf:Description rdf:about="https://www.w3.org/2002/07/owl#sameas">
        <rdf-syntax-ns:type rdf:resource="https://www.w3.org/2002/07/owl#AnnotationProperty"/>
    </rdf:Description>
</rdf:RDF>



<!-- Generated by the OWL API (version 5.1.18) https://github.com/owlcs/owlapi/ -->


